src/main.c
@@ -1,7 +1,28 @@
 #include "list.h"
 
+// list element "allocator"
+
+struct list *get_new_data(void)
+{
+  static struct list list_elems[30];
+  static unsigned int elem_rest = 30;
+  if (elem_rest == 0)
+    return NULL;
+  elem_rest = elem_rest - 1;
+  return &list_elems[elem_rest];
+}
+
+
 int main(void)
 {
+  static struct list *main_list;
+  list_empty(&main_list);
+
+  {
+    struct list *d = get_new_data();
+    d->data = (void *)3;
+    list_insert_front(&main_list, d);
+  }
 
   return 0;
 }
